basic_fallible_transform.thy
@@ -166,6 +166,16 @@ lemma ftrans_does_not_peek_past_end[peek_past_end_simps]:
   by meson
 
 
+\<comment> \<open>Does not consume past char.\<close>
+lemma ftrans_does_not_consume_past_char:
+  assumes "does_not_consume_past_char (parse a) ch"
+  shows "does_not_consume_past_char (parse (ftransform f f' a)) ch"
+  using assms
+  unfolding does_not_consume_past_char_def
+  by (auto simp add: ftransform_has_result)
+
+
+
 
 \<comment> \<open>Well Formed\<close>
 
