basic_one_char.thy
@@ -98,6 +98,13 @@ lemma one_char_does_not_peek_past_end[peek_past_end_simps]:
   by (clarsimp simp add: one_char_has_result)
 
 
+\<comment> \<open>Does not consume past char.\<close>
+lemma one_char_does_not_consume_past_char:
+  shows "does_not_consume_past_char (parse one_char) ch"
+  unfolding does_not_consume_past_char_def
+  by (clarsimp simp add: one_char_has_result)
+
+
 
 \<comment> \<open>Well Formed\<close>
 lemma one_char_well_formed[bi_well_formed_simps]:
