basic_return.thy
@@ -99,6 +99,13 @@ lemma return_does_not_peek_past_end[peek_past_end_simps]:
   by (clarsimp simp add: return_has_result)
 
 
+\<comment> \<open>Does not consume past char.\<close>
+lemma return_does_not_consume_past_char:
+  shows "does_not_consume_past_char (parse (return a)) ch"
+  unfolding does_not_consume_past_char_def
+  by (clarsimp simp add: return_has_result)
+
+
 
 \<comment> \<open>Well Formed\<close>
 lemma b_return_well_formed:
